theories/quoteRecord.v
@@ -60,16 +60,6 @@ Definition over_mien (mien:mutual_inductive_entry) (projs:list ident)
          (mind_entry_private mien)).
 
 
-Definition is_prim_record (decl:mutual_inductive_body) : option (option ident)
-  :=
-    match ind_bodies decl with
-    | (oib :: nil)%list =>
-      match ind_ctors oib with
-      | (((id,_), _) :: nil)%list => Some (Some id) (* Some data is missing wrt to primitivity *)
-      | _ => None
-      end
-    | _ => None
-    end.
 
 Definition mem {A} (eq:A -> A -> bool) (a:A) (l:list A) : bool := isSome (List.find (eq a) l).
 
@@ -92,38 +82,6 @@ Definition over_mib (decl:mutual_inductive_body) (projs:list ident) : mutual_ind
     (List.map (over_oib decl projs) (ind_bodies decl))
     (ind_universes decl).
 
-Definition mind_body_to_entry (decl : mutual_inductive_body)
-  : mutual_inductive_entry.
-Proof.
-  refine {| mind_entry_record := is_prim_record decl;
-            mind_entry_finite := ind_finite decl;
-            mind_entry_params := _;
-            mind_entry_inds := _;
-            mind_entry_universes := decl.(ind_universes);
-            mind_entry_private := None |}.
-  - refine (match List.hd_error decl.(ind_bodies) with
-            | Some i0 => List.rev _
-            | None => nil (* assert false: at least one inductive in a mutual block *)
-            end).
-    pose (typ := decompose_prod i0.(ind_type)).
-    destruct typ as [[names types] _].
-    apply (List.firstn decl.(ind_npars)) in names.
-    apply (List.firstn decl.(ind_npars)) in types.
-    refine (List.combine _ _).
-    exact (List.map get_ident names).
-    exact (List.map LocalAssum types).
-  - refine (List.map _ decl.(ind_bodies)).
-    intros [].
-    refine {| mind_entry_typename := ind_name;
-              mind_entry_arity := remove_arity decl.(ind_npars) ind_type;
-              mind_entry_template := false;
-              mind_entry_consnames := _;
-              mind_entry_lc := _;
-            |}.
-    refine (List.map (fun x => fst (fst x)) ind_ctors).
-    refine (List.map (fun x => remove_arity decl.(ind_npars)
-                                                (snd (fst x))) ind_ctors).
-Defined.
 
 Module test.
   Parameter (X Y Z : Type).
