theories/genDiscriminators.v
@@ -1,9 +1,47 @@
+From mathcomp Require Import ssreflect.seq.
 From Coq Require Import Strings.String.
 From MetaCoq.Template Require Import All.
 From Genxs Require Import metacoq_utils.
 
 
+
 Import MonadNotation.
+
+Section IteriInd.
+  Let ctor_t := (ident × term) × nat.
+  Context (h : inductive -> mutual_inductive_body -> nat -> one_inductive_body -> nat -> ctor_t -> TemplateMonad unit).
+
+
+  Definition oneindbody_iteri
+           (ind : inductive)
+           (mindbody : mutual_inductive_body)
+           (oind_index : nat)
+           (oindbody : one_inductive_body)
+  : TemplateMonad unit :=
+  monad_iteri (h ind mindbody oind_index oindbody) (ind_ctors oindbody).
+
+  Definition mutualindbody_iteri (mindname : qualid)
+  : TemplateMonad unit :=
+    ind <- get_inductive mindname ;;
+    mindbody <- tmQuoteInductive mindname ;;
+    monad_iteri (oneindbody_iteri ind mindbody) (ind_bodies mindbody).
+
+End IteriInd.
+
+
+(** Naming conventions *)
+Section Naming.
+  Context (ctor_id : ident).
+
+  Definition discr_id := "is" ++ ctor_id.
+  Definition discr_class_id := "is_" ++ ctor_id.
+  Definition discr_class_proj_id := "is" ++ ctor_id ++ "_pf".
+  Definition discr_class_ctor_id := "mkIs_" ++ ctor_id.
+  Definition discr_class_Etype_id := discr_class_id ++ "_Etype".
+
+End Naming.
+
+
 
 (** Generation of discrimators *)
 
@@ -13,6 +51,7 @@ Definition qBool :=
 Quote Definition qtrue := true.
 Quote Definition qfalse := false.
 
+Definition lf := String (Ascii.ascii_of_nat 10) EmptyString.
 
 Definition indctor_gen_discriminators
            (debug:bool)
@@ -22,11 +61,11 @@ Definition indctor_gen_discriminators
            (oindbody : one_inductive_body)
            (ctor_index : nat)
            '(((ctor_id, _ty), _arity) : (ident × term) × nat) :=
-  let discr_id := "is" ++ ctor_id in
+  let discr_id := discr_id ctor_id in
+  let ctx := ind_params mindbody in
   let discr_body :=
     let universes := nil (*FIXME*) in
     let npars := ind_npars mindbody in
-    let ctx := ind_params mindbody in
     let ind0 := mkInd indname oind_index in
     let ind shift := mkApps_ctx (tInd ind0 universes) shift ctx in
     let build_branch ctor_k '(((_ , ty),arity): (ident × term) × nat) :=
@@ -48,7 +87,12 @@ Definition indctor_gen_discriminators
   then tmPrint t
   else
     tmMkDefinition discr_id t ;;
-    tmMsg (discr_id ++ " is defined.").
+    let args :=
+        List.fold_left (fun s _ => "{_} " ++ s) ctx "_ : simpl nomatch."
+    in
+    tmMsg (discr_id ++ " is defined. You may want to execute"
+                    ++ lf ++ "Arguments " ++ discr_id ++ " " ++ args).
+
 
 Definition oneindbody_gen_discriminators
            (debug:bool)
@@ -68,9 +112,235 @@ Definition gen_discriminators (debug:bool) (mindname : qualid) (* Is it a kernam
     (oneindbody_gen_discriminators debug mindname mindbody)
     (ind_bodies mindbody).
 
+(** Building discriminator classes *)
+
+Definition build_discr_class
+           (indname : qualid)
+           (mindbody : mutual_inductive_body)
+           (oind_index : nat)
+           (oindbody : one_inductive_body)
+           (ctor_index : nat)
+           '(((ctor_id, _ty), _arity) : (ident × term) × nat)
+           (dicriminator_kn:ident) :=
+  let pr_name := nNamed "principal" in
+  let prop :=
+      tSort (Universe.make'' (Level.lProp, false) nil)
+  in
+
+  let universes := nil (*FIXME*) in
+  let npars := ind_npars mindbody in
+  let ctx := ind_params mindbody in
+  let ind0 := mkInd indname oind_index in
+  let ind shift := mkApps_ctx (tInd ind0 universes) shift ctx in
+
+
+  let discriminator := tConst dicriminator_kn nil in
+  let proj_ty (shift:nat) :=
+      mkApp (tConst "Coq.Init.Datatypes.is_true" nil)
+            (mkApp (mkApps_ctx discriminator (1+shift) ctx) (tRel shift))
+  in
+  let proj := (discr_class_proj_id ctor_id, proj_ty 1) in
+
+  let ctor :=
+      let class_ty :=
+          mkApp (mkApps_ctx (tRel (npars + 2)) 2 ctx) (tRel 1) in
+      let ctor_ty :=
+          it_mkProd_or_LetIn ctx (tProd pr_name (ind 0) (tProd nAnon (* (nNamed "pf") *) (proj_ty 0) class_ty))
+      in
+      (discr_class_ctor_id ctor_id, ctor_ty, 1 (* arity *))
+  in
+
+  let class_body :=
+      Build_one_inductive_body (discr_class_id ctor_id)
+                               (it_mkProd_or_LetIn ctx (tProd pr_name (ind 0) prop))
+                               [:: InProp ; InSet ; InType]
+                               [:: ctor]
+                               [:: proj]
+  in
+  let ind_uvs :=
+      Monomorphic_ctx (LevelSetProp.of_list nil, ConstraintSet.empty)
+  in
+  Build_mutual_inductive_body
+    BiFinite
+    (1 + npars)
+    (mkdecl pr_name None (ind 0) :: ctx)
+    [:: class_body]
+    ind_uvs.
+
+
+Definition indctor_gen_discr_class
+           (debug:bool)
+           (indname : qualid)
+           (mindbody : mutual_inductive_body)
+           (oind_index : nat)
+           (oindbody : one_inductive_body)
+           (ctor_index : nat)
+           ctor
+  :=
+    let '((ctor_id, ty), arity) := ctor in
+    discr_name <- tmEval all (discr_id ctor_id) ;;
+    discr_kn <- get_const discr_name;;
+    let discr_class_mid := build_discr_class indname mindbody oind_index oindbody ctor_index ctor discr_kn in
+    let mindentry := mind_body_to_entry discr_class_mid in
+    if debug then
+      t <- tmEval all discr_class_mid ;;
+      tmPrint t
+    else
+      tmMkInductive mindentry ;;
+      (* class_id <- tmEval all (discr_class_id ctor_id) ;; *)
+      (* tmExistingInstance class_id;; *)
+      tmMsg ("Existing Class " ++ discr_class_id ctor_id ++ ".").
+
+Definition oid_gen_discr_class
+           (debug:bool)
+           (indname : qualid)
+           (mindbody : mutual_inductive_body)
+           (oind_index : nat)
+           (oindbody : one_inductive_body)
+  : TemplateMonad unit :=
+  monad_iteri
+    (indctor_gen_discr_class debug indname mindbody oind_index oindbody)
+    (ind_ctors oindbody).
+
+Definition gen_discr_class (debug:bool) (mindname : qualid) (* Is it a kername ?*)
+  : TemplateMonad unit :=
+  mindbody <- tmQuoteInductive mindname ;;
+  monad_iteri
+    (oid_gen_discr_class debug mindname mindbody)
+    (ind_bodies mindbody).
+
+
+(** Generation of the type of elimination for the discr class *)
+Quote Definition qeq_refl := @eq_refl.
+Quote Definition qFalse := False.
+Quote Definition qeq := @eq.
+
+Definition build_discr_class_Etype
+           (indname : qualid)
+           (mindbody : mutual_inductive_body)
+           (oind_index : nat)
+           (oindbody : one_inductive_body)
+           (ctor_index : nat)
+           '(((ctor_id, _ty), _arity) : (ident × term) × nat)
+           (discrclass_kn:ident) :=
+  let pr_name := nNamed "principal" in
+  let prop := tSort (Universe.make'' (Level.lProp, false) nil) in
+  let pf_inst_name := nNamed "pf_inst" in
+
+  let universes := nil (*FIXME*) in
+  let npars := ind_npars mindbody in
+  let ctx := ind_params mindbody in
+  let ind0 := mkInd indname oind_index in
+  let ind shift := mkApps_ctx (tInd ind0 universes) shift ctx in
+
+  let discrclass_ind := mkInd discrclass_kn 0 in
+  let class_ty shift principal :=
+    mkApp (mkApps_ctx (tInd discrclass_ind [::] (*FIXME*)) shift ctx) principal
+  in
+
+  let body :=
+    let build_branch ctor_k '(((_ , ty),arity): (ident × term) × nat) :=
+      let '(argtys, nargtys) :=
+        let '(_, tys, _) := decompose_prod ty in
+        let argtys := List.skipn npars tys in
+        (fun shift =>mapi (fun i ty => lift shift i ty) argtys, List.length argtys)
+      in
+      let re_ctor shift :=
+        let ctor := tConstruct ind0 ctor_k [::] (* FIXME *) in
+        mkApps (mkApps_ctx ctor (shift+2+nargtys) ctx) (rev [seq tRel i | i <- iota shift nargtys])
+      in
+      let class_ty shift := class_ty (shift+2+nargtys) (re_ctor shift) in
+      let body :=
+        if eq_nat ctor_k ctor_index then
+          (* let refl_ctor := mkApps qeq_refl (ind (nargtys + 2) :: re_ctor :: nil) in *)
+          let refl_ctor := mkApps qeq_refl (qBool :: qtrue :: nil) in
+          let discr_class_ctor := tConstruct discrclass_ind 0 [::] (* FIXME*)in
+          let re_class_ctor := mkApps discr_class_ctor ([seq tRel i | i <- iota (3+nargtys) npars] ++ [:: re_ctor 1 ; refl_ctor]) in
+          mkApps qeq (class_ty 1 :: tRel 0 :: re_class_ctor :: nil)
+        else qFalse
+      in
+      let brnch := build_const (argtys 2) (tLambda pf_inst_name (class_ty 0) body) in
+      (nargtys, brnch)
+    in
+    let branches := utils.mapi build_branch (ind_ctors oindbody) in
+    let motive := tLambda pr_name (ind 2) (tProd pf_inst_name (class_ty 3 (tRel 0)) prop) in
+    tCase (ind0, npars) motive (tRel 1) branches
+  in
+  let comm_cut := tProd pf_inst_name (class_ty 1 (tRel 0)) (mkApp body (tRel 0)) in
+  it_mkLambda_or_LetIn ctx (tLambda pr_name (ind 0) comm_cut).
+
+
+Definition gen_discr_class_Etype (debug:bool) (mindname : qualid)
+  : TemplateMonad unit :=
+  mindbody <- tmQuoteInductive mindname ;;
+  let oid_gen oind_index oindbody :=
+    let ctor_gen ctor_idx ctor :=
+      let '((ctor_id, ty), arity) := ctor in
+      discrclass_name <- tmEval all (discr_class_id ctor_id) ;;
+      discrclass_ind <- get_inductive discrclass_name;;
+      let discr_class_Etype :=
+        build_discr_class_Etype mindname mindbody oind_index oindbody ctor_idx ctor (inductive_mind discrclass_ind)
+      in
+      if debug then t <- tmEval all discr_class_Etype ;; tmPrint t
+      else
+        tmMkDefinition (discr_class_Etype_id ctor_id) discr_class_Etype ;;
+        tmMsg ("Arguments " ++ discr_class_Etype_id ctor_id ++ ".") (*FIXME*)
+    in
+    monad_iteri ctor_gen (ind_ctors oindbody)
+  in
+  monad_iteri oid_gen (ind_bodies mindbody).
 
 (** Tests *)
 Module TestGenDiscriminators.
+  Set Primitive Projections.
+
+  Inductive myBool := myTrue | myFalse.
+  Run TemplateProgram (gen_discriminators false "myBool").
+  Arguments ismyTrue _ : simpl nomatch.
+  Arguments ismyFalse _ : simpl nomatch.
+
+  Run TemplateProgram (gen_discr_class false "myBool").
+  Existing Class is_myTrue.
+  Existing Class is_myFalse.
+
+  Run TemplateProgram (gen_discriminators false "bool").
+  Class is_true0 (b:bool) := mkIs_true0 { istrue_pf0 : istrue b }.
+  Run TemplateProgram (t <- tmQuoteInductive "is_true0";; tmPrint t).
+  Run TemplateProgram (gen_discr_class false "bool").
+  Run TemplateProgram (gen_discr_class_Etype false "bool").
+
+  Run TemplateProgram (gen_discriminators false "option").
+  Class is_none0 {A:Type} (m:option A) := mkIs_None0 { isNone_pf0 : isNone A m }.
+  Run TemplateProgram (t <- tmQuoteInductive "is_none0";; tmPrint t).
+  Class is_Some0 {A:Type} (m:option A) := mkIs_Some0 { isSome_pf0 : isSome A m }.
+  Run TemplateProgram (t <- tmQuoteInductive "is_Some0";; tmPrint t).
+  Run TemplateProgram (gen_discr_class false "option").
+  Existing Class is_Some.
+  Existing Class is_None.
+  Run TemplateProgram (gen_discr_class_Etype false "option").
+
+  Quote Definition is_SomeEty0 := (fun (A:Type) m =>
+    forall H : is_Some A m, (match m with None => fun _ => False | Some v => fun H => H = mkIs_Some A (Some v) eq_refl end) H).
+
+  From Genxs Require Import etaRecord.
+  Run TemplateProgram (gen_eta_instance "is_Some0").
+
+
+  Quote Definition is_someE' := (fun {A} {m:option A} =>
+    match m with
+    | Some y => fun H0 : is_some (Some y) =>
+                f_equal (mkIsSome _ (Some y)) (Eqdep_dec.UIP_refl_bool _ _)
+    | None => fun H0 : is_some None => notF is_some_pf
+    end :
+    forall H : is_some m, (if m is Some v then fun H => H = ⦅v⦆ else fun _ => False) H).
+
+  Run TemplateProgram (gen_discriminators false "prod").
+  Class is_pair0 (A B : Type) (p : A * B) := mkIs_pair0 { ispair_pf0 : ispair A B p }.
+
+  Run TemplateProgram (t <- tmQuoteInductive "is_pair0";; tmPrint t).
+  Run TemplateProgram (gen_discr_class false "prod").
+  Existing Class is_pair.
+
 
   Inductive I (A:Type) := IX : I A | IY : nat -> I A | IZ : forall (x:nat), x+x = 2 -> I A.
 
@@ -79,6 +349,10 @@ Module TestGenDiscriminators.
   Quote Definition qisIX0 := Eval unfold isIX0 in isIX0.
 
   Run TemplateProgram (gen_discriminators false "I").
+  Run TemplateProgram (gen_discr_class false "I").
+  Existing Class is_IX.
+  Existing Class is_IY.
+  Existing Class is_IZ.
 
   From Coq Require Import ssreflect.
 
